more suitable sequential composition, fast build

theories/Compositional_Structures/Basic_Modules/Component_Types/Electoral_Module_Ref.thy
@@ -19,8 +19,8 @@ type_synonym 'a Electoral_Module_Sep = "('a, unit) hashtable
          \<Rightarrow> (('a, unit) hashtable \<times> ('a, unit) hashtable \<times> ('a, unit) hashtable) Heap"
 
 
-abbreviation elec_mod_rel_orig :: "('a \<times> 'a) set \<Rightarrow> 
-  ('a Electoral_Module \<times> 'a Electoral_Module) set" where
+definition elec_mod_rel_orig :: "('b \<times> 'b) set \<Rightarrow> 
+  ('b Electoral_Module \<times> 'b Electoral_Module) set" where
   "elec_mod_rel_orig R \<equiv> \<langle>\<langle>R\<rangle>set_rel , \<langle>\<langle>\<langle>R \<times>\<^sub>r R\<rangle>set_rel\<rangle>list_rel , 
   \<langle>R\<rangle>set_rel \<times>\<^sub>r \<langle>R\<rangle>set_rel \<times>\<^sub>r \<langle>R\<rangle>set_rel\<rangle>fun_rel\<rangle>fun_rel" 
 
@@ -30,11 +30,22 @@ abbreviation elec_mod_rel_orig_nres :: "('a \<times> 'a) set \<Rightarrow>
   "elec_mod_rel_orig_nres R \<equiv> \<langle>\<langle>R\<rangle>set_rel , \<langle>\<langle>\<langle>R \<times>\<^sub>r R\<rangle>set_rel\<rangle>list_rel , 
   \<langle>\<langle>R\<rangle>set_rel \<times>\<^sub>r \<langle>R\<rangle>set_rel \<times>\<^sub>r \<langle>R\<rangle>set_rel\<rangle>nres_rel\<rangle>fun_rel\<rangle>fun_rel" 
 
-abbreviation elec_mod_assn where 
-  "elec_mod_assn R \<equiv> [\<lambda>(a, b).
+abbreviation elec_mod_seprel where 
+  "elec_mod_seprel R \<equiv> [\<lambda>(a, b).
            finite_profile a b]\<^sub>a (alts_set_impl_assn R)\<^sup>k *\<^sub>a 
     (list_assn (ballot_assn R))\<^sup>k 
         \<rightarrow> (result_impl_assn R)"
+
+definition "is_arrayd_list l \<equiv> \<lambda>(a,n). \<exists>\<^sub>Al'. a \<mapsto>\<^sub>a l' * \<up>(n \<le> length l' \<and> l = take n l' \<and> length l'>0)"
+
+find_theorems name:"assn"
+
+definition elec_mod_assn_atom:: 
+  "('a  \<Rightarrow> 'a  \<Rightarrow> assn)
+     \<Rightarrow> 'a::{default, hashable, heap} Electoral_Module \<Rightarrow> 'a::{default, hashable, heap}  Electoral_Module_Sep \<Rightarrow> assn" where
+  "elec_mod_assn_atom R em em_sep \<equiv> emp * \<up>((uncurry em_sep, uncurry (RETURN oo em))
+  \<in> elec_mod_seprel R)"
+  
 
 
 end
