theories/Compositional_Structures/Elect_Composition_Ref.thy
@@ -9,31 +9,38 @@ theory Elect_Composition_Ref
           Sequential_Composition_Ref
 begin
 
-definition elector_opt :: "('a set \<Rightarrow> 'a Profile \<Rightarrow> 'a Result nres) \<Rightarrow> 
+definition elector_opt :: "('a Electoral_Module) \<Rightarrow> 
   'a set \<Rightarrow> 'a Profile \<Rightarrow> 'a Result nres" where
-  "elector_opt m A p \<equiv> do { 
-      (e, r, d) \<leftarrow> m A p;
+    "elector_opt m A p \<equiv> do { 
+      let (e, r, d) = m A p;
       RETURN (e \<union> d,r,{}) }"
 
 lemma elector_opt_correct: 
   fixes m :: "'a Electoral_Module"
-  assumes em_m: "electoral_module m" 
-shows "(uncurry (elector_opt (RETURN oo m)), uncurry (RETURN oo (elector m))) \<in>
+shows "(uncurry (elector_opt (m)), uncurry (RETURN oo (elector m))) \<in>
   [\<lambda> (A, p). finite_profile A p]\<^sub>f (\<langle>Id\<rangle>set_rel \<times>\<^sub>r \<langle>\<langle>Id \<times>\<^sub>r Id\<rangle>set_rel\<rangle>list_rel) \<rightarrow> 
   \<langle>\<langle>Id\<rangle>set_rel \<times>\<^sub>r \<langle>Id\<rangle>set_rel \<times>\<^sub>r \<langle>Id\<rangle>set_rel\<rangle>nres_rel"
   unfolding elector_opt_def
   apply (intro frefI nres_relI) apply clarsimp
-  using assms apply (refine_vcg)
+   apply (refine_vcg)
   by auto
 
-lemma elector_opt_correct_nres: 
+lemma elector_opt_eq:
+  shows "elector_opt \<equiv> (RETURN \<circ>\<circ>\<circ> (elector))"
+  unfolding elector_opt_def elector.simps seqcomp_alt_eq[symmetric]
+  sequential_composition'.simps comp_apply
+  apply auto
+  by (simp add: case_prod_beta')
+  
+
+(*lemma elector_opt_correct_nres: 
   fixes m_opt :: "('a set \<Rightarrow> 'a Profile \<Rightarrow> 'a Result nres)"
 fixes m :: "'a Electoral_Module"
 assumes em_m: "electoral_module m" 
 assumes mref: "(uncurry m_opt, uncurry (RETURN oo m)) \<in>  
   [\<lambda> (A, p). finite_profile A p]\<^sub>f (\<langle>Id\<rangle>set_rel \<times>\<^sub>r \<langle>\<langle>Id \<times>\<^sub>r Id\<rangle>set_rel\<rangle>list_rel) \<rightarrow> 
    \<langle>\<langle>Id\<rangle>set_rel \<times>\<^sub>r \<langle>Id\<rangle>set_rel \<times>\<^sub>r \<langle>Id\<rangle>set_rel\<rangle>nres_rel"
-shows "(uncurry (elector_opt (m_opt)), uncurry (RETURN oo (elector m))) \<in>
+shows "(uncurry (elector_opt (m)), uncurry ((elector m))) \<in>
   [\<lambda> (A, p). finite_profile A p]\<^sub>f (\<langle>Id\<rangle>set_rel \<times>\<^sub>r \<langle>\<langle>Id \<times>\<^sub>r Id\<rangle>set_rel\<rangle>list_rel) \<rightarrow> 
   \<langle>\<langle>Id\<rangle>set_rel \<times>\<^sub>r \<langle>Id\<rangle>set_rel \<times>\<^sub>r \<langle>Id\<rangle>set_rel\<rangle>nres_rel"
   unfolding elector_opt_def
@@ -50,7 +57,41 @@ proof (rename_tac A p, refine_vcg, unfold SPEC_eq_is_RETURN)
            \<le> SPEC (\<lambda>x. (case x of (e, r, d) \<Rightarrow> RETURN (e \<union> d, r, {}))
                         \<le> RETURN (elect m A p \<union> defer m A p, reject m A p, {}))"
     by (simp add: case_prod_beta' order_trans)
-qed
+qed*)
+
+locale Elector_Impl =
+  fixes m :: "'a::{default, heap, hashable} Electoral_Module"
+  fixes m_sep :: "'a::{default, heap, hashable} Electoral_Module_Sep"
+  assumes em_m: "electoral_module m" 
+  assumes m_sep_correct: "(uncurry m_sep, uncurry (RETURN oo m)) \<in> elec_mod_seprel id_assn"
+begin
    
+  lemma this_loc: "Elector_Impl m m_sep " by unfold_locales
+
+  sepref_register m
+
+  declare m_sep_correct[sepref_fr_rules]
+
+schematic_goal elector_sepimpl:
+  "(uncurry ?f2, uncurry (elector_opt m)) \<in> elec_mod_seprel id_assn"
+  unfolding elector_opt_def hs.fold_custom_empty
+  by sepref
+
+concrete_definition elector_sep_uc uses Elector_Impl.elector_sepimpl
+  prepare_code_thms elector_sep_uc_def
+lemmas  elector_sep_ucp_refine = elector_sep_uc.refine[OF this_loc]
+
+schematic_goal elector_sep_curried:
+ "?curried = curry (elector_sep_uc m_sep)" by auto
+
+concrete_definition (in -) elector_sep uses Elector_Impl.elector_sep_curried
+
+  theorem seqcomp_sep_correct:
+  shows "(uncurry (elector_sep m_sep), uncurry (RETURN oo (elector m))) \<in> elec_mod_seprel id_assn"
+    using elector_sep_ucp_refine[FCOMP elector_opt_correct]
+    unfolding elector_sep_def
+    by (simp)
+
+end
 
 end
