theories/Compositional_Structures/Sequential_Composition_Ref.thy
@@ -4,7 +4,7 @@ theory Sequential_Composition_Ref
         Refine_Imperative_HOL.Sepref
 begin
 
-definition seq_opt :: "'a Electoral_Module \<Rightarrow> 
+definition seq_opt :: "'a :: {default, heap, hashable} Electoral_Module \<Rightarrow> 
   'a Electoral_Module
   \<Rightarrow> 'a set \<Rightarrow> 'a Profile \<Rightarrow> 
   'a Result nres" 
@@ -20,7 +20,7 @@ definition seq_opt :: "'a Electoral_Module \<Rightarrow>
    RETURN (e \<union> ne, r \<union> nr, nd) }"
 
 lemma seq_opt_correct: 
-  fixes m n :: "'a Electoral_Module"
+  fixes m n :: "'a :: {default, heap, hashable} Electoral_Module"
   assumes em_m: "electoral_module m" and
   em_n: "electoral_module n"
 shows "(uncurry (seq_opt m n), uncurry (RETURN oo (sequential_composition' m n))) \<in>
@@ -34,10 +34,75 @@ shows "(uncurry (seq_opt m n), uncurry (RETURN oo (sequential_composition' m n))
     by (metis def_presv_fin_prof em_m snd_conv)
   apply (metis defer_in_alts snd_conv subsetD) 
   by (metis def_presv_fin_prof limit_profile.elims snd_conv)
-  
+
+locale Seqcomp_Impl =
+  fixes m n :: "'a :: {default, heap, hashable} Electoral_Module"
+  fixes m_sep n_sep :: "'a :: {default, heap, hashable} Electoral_Module_Sep"
+assumes em_m: "electoral_module m" and
+  em_n: "electoral_module n"
+  assumes m_sep_correct: "(uncurry m_sep, uncurry (RETURN oo m)) \<in> elec_mod_seprel id_assn"
+  assumes n_sep_correct: "(uncurry n_sep, uncurry (RETURN oo n)) \<in> elec_mod_seprel id_assn"
+begin
+
+  lemma this_loc: "Seqcomp_Impl m n m_sep n_sep" by unfold_locales
+
+  sepref_register m
+  sepref_register n
+
+  declare m_sep_correct[sepref_fr_rules]
+  declare n_sep_correct[sepref_fr_rules]
+
+schematic_goal seqcomp_sepimpl:
+  "(uncurry ?f2, uncurry (seq_opt m n)) \<in> elec_mod_seprel id_assn"
+  unfolding seq_opt_def
+  by sepref
+
+concrete_definition (in -) seqcomp_sep_uc uses Seqcomp_Impl.seqcomp_sepimpl
+  prepare_code_thms (in -) seqcomp_sep_uc_def
+lemmas  seqcomp_sep_ucp_refine = seqcomp_sep_uc.refine[OF this_loc]
+
+schematic_goal seqcomp_sepcurried:
+ "?curried = curry (seqcomp_sep_uc m_sep n_sep)" by auto
+
+concrete_definition (in -) seqcomp_sep uses Seqcomp_Impl.seqcomp_sepcurried
+
+theorem seqcomp_sep_correct:
+  shows "(uncurry (seqcomp_sep m_sep n_sep), uncurry (RETURN oo (PR_CONST (m \<triangleright> n)))) 
+\<in> elec_mod_seprel id_assn"
+    using seqcomp_sep_ucp_refine[FCOMP seq_opt_correct, OF em_m em_n]
+    unfolding seqcomp_alt_eq seqcomp_sep_def
+    by (simp)
+
+end
+
+abbreviation comp4 (infixl "oooo" 55) where "f oooo g \<equiv> \<lambda>x. f ooo (g x)"
+
+(*theorem seqcomp_sep_correct [sepref_fr_rules]:
+  shows "(uncurry3 (seqcomp_sep), uncurry3 (RETURN oooo sequential_composition))
+   \<in> [\<lambda> (((m,n),a),b). electoral_module m \<and>
+  electoral_module n \<and> finite_profile a b]\<^sub>a (elec_mod_assn_atom nat_assn)\<^sup>k *\<^sub>a 
+    (elec_mod_assn_atom nat_assn)\<^sup>k  
+    *\<^sub>a (alts_set_impl_assn nat_assn)\<^sup>k *\<^sub>a (list_assn (ballot_assn nat_assn))\<^sup>k 
+        \<rightarrow> (result_impl_assn nat_assn)"
+  apply (intro hfrefI)
+  using Seqcomp_Impl.seqcomp_sep_correct
+  unfolding Seqcomp_Impl_def
+  unfolding hn_refine_def  hfref_def elec_mod_assn_atom_def hfref_def
+  apply (sep_auto simp del: sequential_composition.simps) done
+
+sepref_register "sequential_composition"
+
+declare seqcomp_sep_correct [sepref_fr_rules]
+
+sepref_decl_op seqi: "(uncurry3 sequential_composition)" :: 
+  "\<langle>elec_mod_rel_orig R, \<langle>elec_mod_rel_orig R, elec_mod_rel_orig R\<rangle>fun_rel\<rangle>fun_rel" where 
+  "R = (Id)" apply standard apply (rule nres_relI) unfolding elec_mod_rel_orig_def apply auto
+  done*)
+
 
 abbreviation sequence_opt
-     (infix "\<triangleright>opt" 50) where
-  "m \<triangleright>opt n \<equiv> seq_opt m n"
+     (infix "\<triangleright>sep" 50) where
+  "m \<triangleright>sep n \<equiv> seqcomp_sep m n"
+
 
 end
