theories/Borda_Rule_Ref.thy
@@ -9,26 +9,16 @@ theory Borda_Rule_Ref
           "Compositional_Structures/Elect_Composition_Ref"              
 begin
 
-
-
-sepref_definition borda_rule_sep_direct is "uncurry (elector_opt (RETURN oo borda))"
-  :: "[\<lambda>(x, xa).
-       finite_profile x xa ]\<^sub>a (hs.assn nat_assn)\<^sup>k *\<^sub>a
-             (list_assn (ballot_assn nat_assn))\<^sup>k \<rightarrow> 
-                  result_impl_assn nat_assn"
+sepref_definition borda_rule_sep_direct is "uncurry (elector_opt borda)"
+  :: "elec_mod_seprel nat_assn"                                   
   unfolding elector_opt_def hs.fold_custom_empty
-  apply sepref_dbg_keep
-  done
-
-lemmas elect_comp_borda = elector_opt_correct[OF borda_sound]
-lemmas borda_rule_correct_aux = borda_rule_sep_direct.refine[FCOMP elect_comp_borda]
+  by sepref
 
 lemma borda_rule_direct_correct:
   shows "(uncurry borda_rule_sep_direct, uncurry (RETURN oo (borda_rule)))
-  \<in> elec_mod_assn nat_assn"
-  unfolding borda_rule.simps 
-  using  borda_rule_correct_aux  prod_rel_id_simp set_rel_id hr_comp_Id2
-  by (metis)
+  \<in> elec_mod_seprel nat_assn"
+  using borda_rule_sep_direct.refine 
+    unfolding borda_rule.simps elector_opt_eq .
  
 declare borda_rule_direct_correct [sepref_fr_rules]
 
